src/ldrfpf/LocalPFViewMulti.v
@@ -1,0 +1,203 @@
+Require Import RelationClasses.
+
+From Paco Require Import paco.
+From sflib Require Import sflib.
+
+From PromisingLib Require Import Axioms.
+From PromisingLib Require Import Basic.
+From PromisingLib Require Import DataStructure.
+From PromisingLib Require Import Language.
+From PromisingLib Require Import Loc.
+Require Import Time.
+Require Import Event.
+Require Import View.
+Require Import Cell.
+Require Import Memory.
+Require Import MemoryFacts.
+Require Import TView.
+Require Import Local.
+Require Import Thread.
+Require Import Configuration.
+Require Import Progress.
+Require Import Behavior.
+Require Import Cover.
+Require Import PromiseConsistent.
+Require Import Pred.
+Require Import Trace.
+Require Import JoinedView.
+
+Require Import MemoryProps.
+Require Import OrderedTimes.
+Require SimMemory.
+
+Require Import TimeTraced2.
+Require Import LocalPF.
+Require Import LocalPFThread.
+Require Import LocalPFSimView.
+
+Set Implicit Arguments.
+
+
+
+Lemma PF_sim_configuration_beh L times c_src c_mid c_tgt views prom extra
+      (WO: forall loc, well_ordered (times loc))
+      (INCR: forall nat loc, times loc (incr_time_seq nat))
+      (RACEFRFEE: pf_multi_racefree_view L c_src)
+      (WF_SRC: Configuration.wf c_src)
+      (PFSRC: pf_configuration L c_src)
+      (WF_MID: JConfiguration.wf views c_mid)
+      (WF_TGT: Configuration.wf c_tgt)
+      (SIM: sim_configuration L times (fun _ => True) views prom extra c_src c_mid c_tgt)
+  :
+    behaviors (times_configuration_step_all times) c_tgt <1=
+    behaviors (pf_multi_step L) c_src.
+Proof.
+  i. ginduction PR; i.
+  { dep_inv SIM. econs 1. ii. ss.
+    specialize (THSPF tid). specialize (THSJOIN tid).
+    setoid_rewrite FIND in THSPF. unfold option_rel in *. des_ifs.
+    dep_inv THSPF. dep_inv THSJOIN.
+    eapply TERMINAL in Heq0. des. splits; auto.
+    inv THREAD. inv LOCAL. inv LOCAL0. ss. subst.
+    econs. exploit sim_promise_bot; eauto. eapply Memory.ext.
+    i. specialize (PROMISES0 loc ts). erewrite Memory.bot_get in *.
+    inv PROMISES0; ss. }
+  { inv STEP.
+    destruct (classic (List.Forall
+                         (fun the => no_read_msgs
+                                       (all_promises (fun tid' => tid <> tid') prom)
+                                       (snd the)) (tr))).
+    { destruct (classic (List.Forall
+                           (fun the => no_read_msgs
+                                         (all_promises (fun tid' => tid <> tid') prom)
+                                         (snd the)) (tr_cert))).
+      { exploit (step_sim_configuration); eauto.
+        { instantiate (1:=true). ss. }
+        i. des. unguard. des; ss. dep_inv STEPSRC.
+        econs 2; eauto.
+        { econs; eauto. }
+        { eapply IHPR; try apply SIM0; eauto.
+          { eapply multi_steps_pf_multi_racefree_view; eauto. econs; eauto. econs. }
+          { eapply pf_step_trace_future; eauto. }
+          { eapply pf_step_trace_future; eauto. }
+          { eapply JConfiguration.step_future; eauto. }
+          { eapply times_configuration_step_future; eauto. }
+        }
+      }
+      { exploit promise_read_race_certfication; eauto. i. des; clarify. }
+    }
+    { exploit promise_read_race; eauto. i. des; clarify. }
+  }
+  { inv STEP.
+    destruct (classic (List.Forall
+                         (fun the => no_read_msgs
+                                       (all_promises (fun tid' => tid <> tid') prom)
+                                       (snd the)) (tr))).
+    { destruct (classic (List.Forall
+                           (fun the => no_read_msgs
+                                         (all_promises (fun tid' => tid <> tid') prom)
+                                         (snd the)) (tr_cert))).
+      { exploit step_sim_configuration; eauto.
+        { instantiate (1:=true). ss. }
+        i. des. unguard. des; ss.
+        { dep_inv STEPSRC. econs 3; eauto. econs; eauto. }
+        { dep_inv STEPSRC. econs 3; eauto. econs; eauto. }
+      }
+      { exploit promise_read_race_certfication; eauto. i. des; clarify. }
+    }
+    { exploit promise_read_race; eauto. i. des; clarify. }
+  }
+  { inv STEP.
+    destruct (classic (List.Forall
+                         (fun the => no_read_msgs
+                                       (all_promises (fun tid' => tid <> tid') prom)
+                                       (snd the)) (tr))).
+    { destruct (classic (List.Forall
+                           (fun the => no_read_msgs
+                                         (all_promises (fun tid' => tid <> tid') prom)
+                                         (snd the)) (tr_cert))).
+      { exploit step_sim_configuration; eauto.
+        { instantiate (1:=true). ss. }
+        i. des. ss. dep_inv STEPSRC.
+        { econs 4; eauto.
+          { econs; eauto. }
+          { destruct x0; ss. des.
+            eapply IHPR; try apply SIM0; eauto.
+            { eapply multi_steps_pf_multi_racefree_view; eauto. econs; eauto. econs. }
+            { eapply pf_step_trace_future; eauto. }
+            { eapply pf_step_trace_future; eauto. }
+            { eapply JConfiguration.step_future; eauto. }
+            { eapply times_configuration_step_future; eauto. }
+          }
+        }
+        { destruct x0; ss. des.
+          eapply IHPR; try apply SIM0; eauto.
+          { eapply JConfiguration.step_future; eauto. }
+          { eapply times_configuration_step_future; eauto. }
+        }
+      }
+      { exploit promise_read_race_certfication; eauto. i. des; clarify. }
+    }
+    { exploit promise_read_race; eauto. i. des; clarify. }
+  }
+Qed.
+
+
+Theorem local_DRFPF L s
+        (RACEFRFEE: pf_multi_racefree_view L (Configuration.init s))
+  :
+    behaviors Configuration.step (Configuration.init s) <1=
+    behaviors (pf_multi_step L) (Configuration.init s).
+Proof.
+  i. eapply times_configuration_step_same_behaviors in PR; cycle 1.
+  { eapply Configuration.init_wf. }
+  des. eapply PF_sim_configuration_beh; eauto.
+  { eapply Configuration.init_wf. }
+  { eapply configuration_init_pf. }
+  { eapply JConfiguration.init_wf. }
+  { eapply Configuration.init_wf. }
+  instantiate (1:=s). instantiate (1:=bot4). instantiate (1:=bot3). econs; eauto.
+  { i. unfold Threads.init. repeat erewrite IdentMap.Facts.map_o.
+    unfold option_map. des_ifs. ss. econs. econs.
+    econs; ss. i. erewrite Memory.bot_get. destruct (classic (L loc)).
+    { econs 1; eauto. }
+    { econs 2; eauto.  }
+  }
+  { i. unfold Threads.init. repeat erewrite IdentMap.Facts.map_o.
+    unfold option_map. des_ifs. ss. econs. econs.
+    { refl. }
+    { ii. erewrite Memory.bot_get. econs. }
+  }
+  { i. splits; ss. }
+  { econs.
+    { i. unfold Memory.init, Memory.get. erewrite Cell.init_get. des_ifs.
+      { econs 2; eauto.
+        { ii. inv H. ss. }
+        { ii. inv H. ss. }
+        { refl. }
+        { i. apply eq_lb_time. }
+      }
+      { econs.
+        { ii. inv H. ss. }
+        { ii. inv H. ss. }
+      }
+    }
+    { i. inv EXTRA. ss. }
+  }
+  { refl. }
+  { i. unfold JConfiguration.init_views. des_ifs. econs; eauto.
+    eapply Memory.closed_view_bot. eapply Memory.init_closed. }
+  { refl. }
+  { ii. unfold Memory.init, Memory.get in GET. erewrite Cell.init_get in GET.
+    des_ifs. auto. }
+  { i. unfold Threads.init in GET. erewrite IdentMap.Facts.map_o in GET.
+    unfold option_map in GET. des_ifs. dep_clarify. ii. ss. eexists [], _. splits; auto.
+    { refl. }
+    { right. ss. }
+  }
+  { i. unfold Threads.init in GET. erewrite IdentMap.Facts.map_o in GET.
+    unfold option_map in GET. des_ifs. dep_clarify. ii. ss. eexists [], _. splits; auto.
+    { refl. }
+    { right. ss. }
+  }
+Qed.
